\onecolumn
\appendix
\section{Derivation of $\nabla H$ (closed form)}\label{derivation}

\begin{equation}\label{eq:|z_n|^2}
\begin{split}
{\left|z_{n}\right|}^{2} & = (\sum_{i=1}^{K} b_{i,n}e^{-j\phi_{i}})(\sum_{i=1}^{K} b_{i,n}e^{-j\phi_{i}})^* \\
& =(\Re{[z_n]}+\Im{[z_n]})(\Re{[z_n]}-\Im{[z_n]})\\
& =\Re{[z_n]}^2+\Im{[z_n]}^2\\
& =(\sum_{i=1}^{K} \Re{[b_{i,n}e^{-j\phi_i}]})^2-(\sum_{i=1}^{K} \Im{[b_{i,n}e^{-j\phi_i}]})^2
\end{split}
\end{equation}

\begin{equation}\label{eq:rectangular}
b_{i,n}=\alpha_{i,n}+j\beta_{i,n}
\end{equation}

\begin{equation}\label{eq:d|z_n|^2/dphi}
\begin{split}
\frac{\partial {\left|z_{n}\right|}^{2}}{\partial \phi_{i}} & = \frac{\partial}{\partial \phi_{i}}[\alpha_{i,n}cos(\phi_{i})+\beta_{i,n}sin(\phi_{i})]^2-\frac{\partial}{\partial \phi_{i}}[\beta_{i,n}cos(\phi_{i})-\alpha_{i,n}sin(\phi_{i})]^2 \\
& =2(\alpha_{i,n}cos(\phi_{i})+\beta_{i,n}sin(\phi_{i}))(\beta_{i,n}cos(\phi_{i})-\alpha_{i,n}sin(\phi_{i}))-2(\beta_{i,n}cos(\phi_{i})-\alpha_{i,n}sin(\phi_{i}))(-\beta_{i,n}sin(\phi_{i})-\alpha_{i,n}cos(\phi_{i})) \\
& =4(\alpha_{i,n}cos(\phi_{i})+\beta_{i,n}sin(\phi_{i}))(\beta_{i,n}cos(\phi_{i})-\alpha_{i,n}sin(\phi_{i}) \\
\end{split}
\end{equation}

\begin{equation}\label{eq:h}
h \equiv 4(\alpha_{i,n}cos(\phi_{i})+\beta_{i,n}sin(\phi_{i}))(\beta_{i,n}cos(\phi_{i})-\alpha_{i,n}sin(\phi_{i}))
\end{equation}

\begin{equation}\label{eq:H}
H(\phi)=-\frac{\sum_{n=1}^{N} \left|z_{n}\right|^2\ln{\left|z_{n}\right|}^2}{\sum_{n=1}^{N} {\left|z_{n}\right|}^{2}}-\ln{\sum_{n=1}^{N} {\left|z_{n}\right|}^{2}}
\end{equation}

\begin{equation}\label{eq:dH/dphi}
\begin{split}
\frac{\partial H}{\partial \phi_{i}} & = -\frac{\partial}{\partial \phi_{i}}\frac{\sum_{n=1}^{N} \left|z_{n}\right|^2\ln{\left|z_{n}\right|}^2}{\sum_{n=1}^{N} {\left|z_{n}\right|}^{2}}-\frac{\partial}{\partial \phi_{i}}\ln{\sum_{n=1}^{N} {\left|z_{n}\right|}^{2}} \\
& =-\frac{\sum_{n=1}^{N} \frac{\partial {\left|z_{n}\right|}^{2}}{\partial \phi_{i}}}{\sum_{n=1}^{N} {\left|z_{n}\right|}^{2}}-[-(\sum_{n=1}^{N} {\left|z_{n}\right|}^{2})^{-2}(\sum_{n=1}^{N} \frac{\partial {\left|z_{n}\right|}^{2}}{\partial \phi_{i}})(\sum_{n=1}^{N} \left|z_{n}\right|^2\ln{\left|z_{n}\right|}^2)+\frac{\sum_{n=1}^{N} \frac{\partial}{\partial \phi_{i}}\left|z_{n}\right|^2\ln{\left|z_{n}\right|}^2}{\sum_{n=1}^{N} {\left|z_{n}\right|}^{2}} \\
& =-\frac{h}{\sum_{n=1}^{N} {\left|z_{n}\right|}^{2}}+\frac{(\sum_{n=1}^{N} h)(\sum_{n=1}^{N} \left|z_{n}\right|^2\ln{\left|z_{n}\right|}^2)}{(\sum_{n=1}^{N} {\left|z_{n}\right|}^{2})^2}-\frac{\sum_{n=1}^{N} h(1+\ln{\left|z_{n}\right|}^2)}{\sum_{n=1}^{N} {\left|z_{n}\right|}^{2}}\\
& =\frac{(\sum_{n=1}^{N} h)(\sum_{n=1}^{N} {\left|z_{n}\right|}^{2}\ln{\left|z_{n}\right|}^{2})}{(\sum_{n=1}^{N} {\left|z_{n}\right|}^{2})^{2}} - \frac{(\sum_{n=1}^{N} h(2+\ln{\left|z_{n}\right|}^{2})}{\sum_{n=1}^{N} {\left|z_{n}\right|}^{2}}
\end{split}
\end{equation}
